Test/civl/alloc-mem.bpl
@@ -31,7 +31,7 @@ Main ()
   var {:layer 1,2} {:linear "mem"} l:lmap;
   var i:int;
   while (*)
-  invariant {:yields} {:layer 1,2} {:yield_invariant "Yield"} {:yield_invariant "Dummy"} true;
+  invariant {:yields} {:layer 1,2} {:yield_loop "Yield"} true;
   {
     call  l, i := Alloc();
     async call Thread(l, i);
@@ -52,7 +52,7 @@ requires {:layer 2} dom(local_in)[i];
   call o := Read(local, i);
   assert {:layer 2} o == 42;
   while (*)
-  invariant {:yields} {:layer 1,2} {:yield_invariant "Yield"} {:yield_invariant "Dummy"} true;
+  invariant {:yields} {:layer 1,2} {:yield_loop "Yield"} true;
   {
     call l, y := Alloc();
     call l := Write(l, y, 42);
@@ -153,8 +153,6 @@ requires PoolInv(unallocated, pool);
 procedure {:yield_invariant} {:layer 1} YieldMem ({:layer 1} {:linear "mem"} l:lmap, i:int);
 requires PoolInv(unallocated, pool);
 requires dom(l)[i] && map(l)[i] == mem[i];
-
-procedure {:yield_invariant} {:layer 2} Dummy();
 
 var {:layer 1, 2} {:linear "mem"} pool:lmap;
 var {:layer 0, 1} mem:[int]int;
